proofs/transform/eliminate_algebraic.v
@@ -594,63 +594,442 @@ Proof.
     apply a_convert_all_f_equiv.
 Qed.
 
+(*Part 6: Semantics*)
 
+(*TODO move and replace former*)
+Definition gen_name_wf {b: bool} (t: gen_term b) : Prop :=
+  match b return gen_term b -> Prop with
+  | true => term_name_wf
+  | false => fmla_name_wf
+  end t.
 
-(*TODO: move all of these (plus ones in Denotational)*)
-Lemma wf_tfun {f: funsym} {tys: list vty} {tms: list term}
-  (Hwf: term_wf (Tfun f tys tms)):
-  Forall term_wf tms.
+(*TODO: move, copied from elim_def*)
+Definition gen_bnd {b: bool} (t: gen_term b) : list vsymbol :=
+  match b return gen_term b -> list vsymbol with
+  | true => tm_bnd
+  | false => fmla_bnd
+  end t.
+
+Lemma gen_name_wf_eq {b: bool} (t: gen_term b) :
+  gen_name_wf t <->
+  NoDup (map fst (gen_bnd t)) /\ disj (map fst (gen_fv t)) (map fst (gen_bnd t)).
 Proof.
-  unfold term_wf in Hwf. simpl in Hwf.
-  rewrite Forall_forall. intros t Hint.
-  unfold term_wf. destruct Hwf as [Hnodup Hfb].
-  split.
-  - eapply in_concat_NoDup; [apply vsymbol_eq_dec | apply Hnodup |].
-    rewrite in_map_iff. exists t; auto.
-  - intros x [Hinx1 Hinx2].
-    apply (Hfb x). simpl_set. rewrite in_concat.
-    split; eauto.
-    exists (tm_bnd t); split; auto. rewrite in_map_iff. exists t; auto.
+  destruct b; reflexivity.
 Qed.
 
-Lemma wf_tlet {tm1 tm2: term} {x} (Hwf: term_wf (Tlet tm1 x tm2)):
-  term_wf tm1 /\ term_wf tm2.
+Definition gen_fun {b: bool} (s: gen_sym b) (tys: list vty) (tms: list term) : gen_term b :=
+  match b return gen_sym b -> gen_term b with
+  | true => fun f => Tfun f tys tms
+  | false => fun p => Fpred p tys tms
+  end s.
+
+Lemma gen_fun_bnd {b: bool} (s: gen_sym b) (tys: list vty) (tms: list term):
+  gen_bnd (gen_fun s tys tms) = concat (map tm_bnd tms).
+Proof. destruct b; reflexivity. Qed.
+
+Lemma gen_fun_fv {b: bool} (s: gen_sym b) (tys: list vty) (tms: list term):
+  gen_fv (gen_fun s tys tms) = big_union vsymbol_eq_dec tm_fv tms.
+Proof. destruct b; reflexivity. Qed.
+
+Lemma wf_genfun (b: bool) {s: gen_sym b} {tys: list vty} {tms: list term}
+  (Hwf: gen_name_wf (gen_fun s tys tms)):
+  Forall term_name_wf tms.
 Proof.
-  unfold term_wf in Hwf |- *. simpl in Hwf. destruct Hwf as [Hnodup Hfb].
+  rewrite gen_name_wf_eq in Hwf. unfold term_name_wf.
+  rewrite gen_fun_bnd, gen_fun_fv in Hwf.
+  rewrite Forall_forall. intros t Hint.
+  destruct Hwf as [Hnodup Hfb].
+  rewrite concat_map in Hnodup.
+  split.
+  - eapply in_concat_NoDup; [apply string_dec | apply Hnodup |].
+    rewrite in_map_iff. exists (tm_bnd t); rewrite in_map_iff; eauto.
+  - intros x [Hinx1 Hinx2].
+    apply (Hfb x).
+    split; [rewrite in_map_big_union|].
+    + simpl_set. eauto. Unshelve. exact string_dec.
+    + rewrite concat_map, !map_map. 
+      rewrite in_concat. eexists. split; [| apply Hinx2].
+      rewrite in_map_iff. eauto.
+Qed.
+
+Lemma gen_let_bnd  {b: bool} {tm1: term} {tm2: gen_term b} {x}:
+  gen_bnd (gen_let x tm1 tm2) = x :: tm_bnd tm1 ++ gen_bnd tm2.
+Proof. destruct b; reflexivity. Qed.
+
+Lemma gen_let_fv  {b: bool} {tm1: term} {tm2: gen_term b} {x}:
+  gen_fv (gen_let x tm1 tm2) = 
+    union vsymbol_eq_dec (tm_fv tm1) (remove vsymbol_eq_dec x (gen_fv tm2)).
+Proof. destruct b; reflexivity. Qed.
+
+(*TODO: move*)
+(*NOTE: can't get iff unless injective*)
+Lemma in_map_remove {B C: Type} (f: B -> C) eq_dec l y x:
+  In x (map f l) /\ f y <> x ->
+  In x (map f (remove eq_dec y l)).
+Proof.
+  rewrite !in_map_iff. setoid_rewrite in_remove_iff.
+  intros [[x1 [Hx Hinx1]] Hnot]; subst.
+  exists x1; split_all; auto. intro C1; subst; contradiction.
+Qed.
+
+Lemma in_map_remove_all {B C: Type} (f: B -> C) eq_dec l1 l2 x:
+  In x (map f l2) /\ ~ In x (map f l1) ->
+  In x (map f (remove_all eq_dec l1 l2)).
+Proof.
+  rewrite !in_map_iff. setoid_rewrite <- remove_all_elts.
+  intros [[x1 [Hx Hinx1]] Hnot]; subst.
+  exists x1; split_all; auto. intro C1; subst.
+  apply Hnot. exists x1; auto.
+Qed.
+
+Lemma wf_genlet (b: bool) {tm1: term} {tm2: gen_term b} {x} 
+  (Hwf: gen_name_wf (gen_let x tm1 tm2)):
+  term_name_wf tm1 /\ gen_name_wf tm2.
+Proof.
+  rewrite gen_name_wf_eq in Hwf |- *. unfold term_name_wf.
+  rewrite gen_let_bnd, gen_let_fv in Hwf.
+  destruct Hwf as [Hnodup Hfb].
   inversion Hnodup as [| ? ? Hnotin Hn2]; subst.
+  rewrite map_app in Hn2.
   apply NoDup_app in Hn2. destruct Hn2 as [Hn1 Hn2].
   split_all; auto; intros y [Hiny1 Hiny2]; apply (Hfb y);
-  simpl_set; rewrite in_app_iff; auto.
-  split; auto. right. split; auto.
-  intro C; subst. apply Hnotin. rewrite in_app_iff; auto.
+  rewrite in_map_union; simpl_set; simpl; rewrite map_app, in_app_iff; auto.
+  split; auto. right. apply in_map_remove. split; auto.
+  intro C; subst. apply Hnotin. rewrite map_app, in_app_iff; auto.
 Qed.
 
-Lemma wf_tif {f t1 t2} (Hwf: term_wf (Tif f t1 t2)):
-  fmla_wf f /\ term_wf t1 /\ term_wf t2.
+(*TODO move*)
+Definition gen_if {b: bool} (f: formula) (t1 t2: gen_term b) : gen_term b :=
+  match b return gen_term b -> gen_term b -> gen_term b with
+  | true => fun t1 t2 => Tif f t1 t2
+  | false => fun f1 f2 => Fif f f1 f2
+  end t1 t2.
+
+Lemma gen_if_bnd  {b: bool} (f: formula) (t1 t2: gen_term b):
+  gen_bnd (gen_if f t1 t2) = fmla_bnd f ++ gen_bnd t1 ++ gen_bnd t2.
+Proof. destruct b; reflexivity. Qed.
+
+Lemma gen_if_fv  {b: bool} (f: formula) (t1 t2: gen_term b):
+  gen_fv (gen_if f t1 t2) = 
+    union vsymbol_eq_dec (fmla_fv f) 
+      (union vsymbol_eq_dec (gen_fv t1) (gen_fv t2)).
+Proof. destruct b; reflexivity. Qed.
+
+Lemma wf_genif (b : bool) {f} {t1 t2 : gen_term b} 
+  (Hwf: gen_name_wf (gen_if f t1 t2)):
+  fmla_name_wf f /\ gen_name_wf t1 /\ gen_name_wf t2.
 Proof.
-  unfold term_wf, fmla_wf in *. simpl in Hwf.
+  rewrite !gen_name_wf_eq in Hwf |- *.
+  rewrite gen_name_wf_eq. unfold fmla_name_wf.
+  rewrite gen_if_bnd, gen_if_fv in Hwf.
   destruct Hwf as [Hnodup Hfb].
+  rewrite !map_app in Hnodup, Hfb.
   apply NoDup_app in Hnodup.
   destruct Hnodup as [Hn1 Hn2].
   apply NoDup_app in Hn2.
   destruct Hn2 as [Hn2 Hn3].
+  unfold disj in Hfb.
   do 2 (setoid_rewrite in_app_iff in Hfb).
-  split_all; auto; intros x [Hinx1 Hinx2]; apply (Hfb x); simpl_set; auto.
+  split_all; auto; intros x [Hinx1 Hinx2]; apply (Hfb x);
+  rewrite !in_map_union; simpl_set; auto.
 Qed.
-(*
-(*1.5: Free vars*)
-
-(*I think it is sufficient: every free var in rewriteT is also in t?
-  Or do we need iff?
-  Difficulty is from compile_match_single - need to show that 
-  free vars of resulting matrix are (tm_fv t) \ (big_union pat_fv ps)
-  for row ps -> t
-  under simplify, this still holds
-  so we might be able to do iff*)
-Lemma rewrite_free_vars
 
 
-(*2: Semantics*)
+Lemma gen_match_bnd {b: bool} (t: term) (ty: vty) (ps: list (pattern * gen_term b)):
+  gen_bnd (gen_match t ty ps) = 
+    tm_bnd t ++ concat (map (fun p => pat_fv (fst p) ++ gen_bnd (snd p)) ps).
+Proof. destruct b; reflexivity. Qed.
+
+
+Lemma gen_match_fv {b: bool} (t: term) (ty: vty) (ps: list (pattern * gen_term b)):
+  gen_fv (gen_match t ty ps) =
+  union vsymbol_eq_dec (tm_fv t)
+    (big_union vsymbol_eq_dec
+    (fun x => remove_all vsymbol_eq_dec (pat_fv (fst x))
+      (gen_fv (snd x))) ps).
+Proof. destruct b; reflexivity. Qed.
+
+Lemma wf_genmatch (b: bool) {tm ty} {ps: list (pattern * gen_term b)} 
+  (Hwf: gen_name_wf (gen_match tm ty ps)):
+  term_name_wf tm /\ Forall (fun x => gen_name_wf (snd x)) ps.
+Proof.
+  rewrite gen_name_wf_eq in Hwf.
+  unfold term_name_wf. 
+  rewrite gen_match_bnd, gen_match_fv in Hwf.
+  rewrite !map_app in Hwf.
+  destruct Hwf as [Hn Hdisj].
+  apply NoDup_app_iff in Hn.
+  destruct Hn as [Hn1 [Hn2  [Hn12 _]]].
+  split_all; auto.
+  - eapply disj_sublist_lr. apply Hdisj.
+    intros x Hinx. rewrite in_map_union. auto.
+    apply sublist_app_l.
+  - rewrite Forall_forall. intros x Hinx.
+    rewrite gen_name_wf_eq.
+    rewrite concat_map in Hn2.
+    assert (Hn3:
+      NoDup (map fst (pat_fv (fst x)) ++ map fst (gen_bnd (snd x)))).
+    {
+      eapply in_concat_NoDup; [apply string_dec | apply Hn2 |].
+      rewrite in_map_iff. eexists.
+      rewrite <- map_app. split; [reflexivity|]. 
+      rewrite in_map_iff; eauto.
+    }
+    split.
+    + apply NoDup_app in Hn3. apply Hn3.
+    + intros y [Hiny1 Hiny2].
+      (*Because in [tm_bnd], cannot be in [pat_fv]*)
+      assert (Hnotin: ~ In y (map fst (pat_fv (fst x)))). {
+        intro C.
+        apply NoDup_app_iff in Hn3.
+        apply Hn3 in C; auto; contradiction.
+      }
+      apply (Hdisj y). split.
+      * rewrite in_map_union. right.
+        rewrite in_map_big_union with (eq_dec1:=string_dec).
+        simpl_set. exists x. split; auto.
+        apply in_map_remove_all. auto.
+      * rewrite in_app_iff. right. rewrite concat_map, map_map, in_concat.
+        eexists. split; [rewrite in_map_iff; eexists; split; [| apply Hinx]; reflexivity |].
+        rewrite map_app, in_app_iff; auto.
+Qed.
+
+Lemma wf_teps {f v} (Hwf: term_name_wf (Teps f v)):
+  fmla_name_wf f.
+Proof.
+  unfold term_name_wf in Hwf; unfold fmla_name_wf. simpl in *.
+  destruct Hwf as [Hn1 Hdisj].
+  inversion Hn1; subst. split; auto.
+  intros x [Hinx1 Hinx2].
+  assert (x <> fst v) by (intro C; subst; contradiction).
+  apply (Hdisj x); split.
+  - apply in_map_remove. auto.
+  - simpl. auto.
+Qed.
+
+Lemma wf_fquant {q v f} (Hwf: fmla_name_wf (Fquant q v f)):
+  fmla_name_wf f.
+Proof.
+  unfold fmla_name_wf in *; simpl in *.
+  destruct Hwf as [Hn1 Hdisj].
+  inversion Hn1; subst. split; auto.
+  intros x [Hinx1 Hinx2].
+  assert (x <> fst v) by (intro C; subst; contradiction).
+  apply (Hdisj x); split.
+  - apply in_map_remove. auto.
+  - simpl. auto.
+Qed.
+
+Lemma wf_feq {ty t1 t2} (Hwf: fmla_name_wf (Feq ty t1 t2)):
+  term_name_wf t1 /\ term_name_wf t2.
+Proof.
+  unfold term_name_wf, fmla_name_wf in *; simpl in *.
+  rewrite map_app in Hwf.
+  destruct Hwf as [Hn1 Hdisj].
+  apply NoDup_app in Hn1. destruct Hn1 as [Hn1 Hn2]. split_all; auto;
+  eapply disj_sublist_lr; try solve[apply Hdisj];
+  try solve[apply sublist_app_r]; try solve[apply sublist_app_l];
+  intros x Hinx; apply in_map_union; auto.
+Qed.
+
+Lemma wf_fbinop {b f1 f2} (Hwf: fmla_name_wf (Fbinop b f1 f2)):
+  fmla_name_wf f1 /\ fmla_name_wf f2.
+Proof.
+  unfold fmla_name_wf in *; simpl in *.
+  rewrite map_app in Hwf.
+  destruct Hwf as [Hn1 Hdisj].
+  apply NoDup_app in Hn1. destruct Hn1 as [Hn1 Hn2]. split_all; auto;
+  eapply disj_sublist_lr; try solve[apply Hdisj];
+  try solve[apply sublist_app_r]; try solve[apply sublist_app_l];
+  intros x Hinx; apply in_map_union; auto.
+Qed.
+
+Lemma wf_fnot {f} (Hwf: fmla_name_wf (Fnot f)):
+  fmla_name_wf f.
+Proof.
+  unfold fmla_name_wf in *; simpl in *; auto.
+Qed.
+
+
+Lemma disj_sublist2 {A: Type} (l1 l2 l3: list A):
+  sublist l1 l2 ->
+  disj l2 l3 ->
+  disj l1 l3.
+Proof.
+  unfold sublist, disj. intros Hsub Hdisj x [Hinx1 Hinx2].
+  apply (Hdisj x); auto.
+Qed.
+
+Lemma Forall2_map_iff {A B: Type} (f: A -> B) 
+  (P: A -> B -> Prop) (l: list A):
+  Forall2 P l (map f l) <-> Forall (fun x => P x (f x)) l.
+Proof.
+  induction l as [| h t IH]; simpl; [split; constructor|].
+  destruct IH as [IH1 IH2].
+  split; intros Hall; inversion Hall; constructor; auto.
+Qed.
+Check match_rep'.
+(*Check match_rep.*)
+Lemma match_rep_ext {gamma} (gamma_valid: valid_context gamma)
+  pd pdf pf vt vv b (ty: gen_type b) ty1 d (ps1 ps2 : list (pattern * gen_term b))
+  Htyps1 Htyps2 Htms1 Htms2
+  (Hfst: map fst ps1 = map fst ps2)
+  (Hall: Forall2 (fun x y => forall vv ty Hty Hty2, 
+    gen_rep gamma_valid pd pdf pf vt vv ty (snd x) Hty = 
+    gen_rep gamma_valid pd pdf pf vt vv ty (snd y) Hty2) ps1 ps2):
+  match_rep' gamma_valid b pd pdf pf vt vv ty ty1 d ps1 Htyps1 Htms1 =
+  match_rep' gamma_valid b pd pdf pf vt vv ty ty1 d ps2 Htyps2 Htms2.
+Proof.
+  revert Htyps1 Htyps2 Htms1 Htms2. generalize dependent ps2.
+  induction ps1 as [|p1 t1 IH]; intros [| p2 t2]; auto; intros Hfst Hall; inversion Hall.
+  intros. simpl.
+  destruct p1 as [p1 tm1]. destruct p2 as [p2 tm2].
+  simpl in *; subst. inversion Hfst; subst.
+  rewrite match_val_single_irrel with (Hval2:=(Forall_inv Htyps2)).
+  destruct_match_single l1 Hmatch; auto.
+Qed.
+
+Definition gen_rewrite {b: bool} (t: gen_term b) : gen_term b :=
+  match b return gen_term b -> gen_term b with
+  | true => rewriteT
+  | false => rewriteF
+  end t.
+
+(*TODO: move (from Exhaustive)*)
+Lemma gen_match_typed_inv gamma b (tm: term) (ty1: vty) (ps: list (pattern * gen_term b))
+  (ty2: gen_type b):
+  @gen_typed gamma b (gen_match tm ty1 ps) ty2 ->
+  term_has_type gamma tm ty1 /\
+  Forall (fun x => pattern_has_type gamma (fst x) ty1 /\  
+    @gen_typed gamma b (snd x) ty2) ps /\
+  isSome (compile_bare_single b tm ty1 ps).
+Proof.
+  destruct b; intros Htyped; inversion Htyped; subst; split_all; auto;
+  rewrite Forall_forall; intros x Hinx; split; simpl in *; eauto.
+Qed.
+
+Lemma gen_rewrite_typed (b: bool) 
+  {gamma} (gamma_valid: valid_context gamma) (t: gen_term b)
+  (ty: gen_type b):
+  @gen_typed gamma b t ty ->
+  @gen_typed gamma b (gen_rewrite t) ty.
+Proof.
+  destruct b; [apply rewriteT_typed|apply rewriteF_typed]; assumption.
+Qed.
+
+(*Prove interesting case (match) separately, so we can generalize*)
+Lemma rewrite_rep_match_case (b: bool) {gamma} 
+  (gamma_valid: valid_context gamma)
+  (pd: pi_dom) (pdf: pi_dom_full gamma pd)
+  (pf: pi_funpred gamma_valid pd pdf)
+  (vt: val_typevar)
+  (tm: term) (ty: vty) (ps: list (pattern * gen_term b))
+  (IHtm: forall (vv : val_vars pd vt) (ty : vty) (Hty1 : term_has_type gamma tm ty)
+    (Hty2 : term_has_type gamma (rewriteT tm) ty),
+    term_name_wf tm ->
+    term_rep gamma_valid pd pdf vt pf vv (rewriteT tm) ty Hty2 =
+    term_rep gamma_valid pd pdf vt pf vv tm ty Hty1)
+  (IHps: Forall
+    (fun (tm: gen_term b) =>
+    forall (vv : val_vars pd vt) (ty : gen_type b) (Hty1 : @gen_typed gamma b tm ty)
+    (Hty2 : @gen_typed gamma b (gen_rewrite tm) ty),
+    gen_name_wf tm ->
+    gen_rep gamma_valid pd pdf pf vt vv ty (gen_rewrite tm) Hty2 =
+    gen_rep gamma_valid pd pdf pf vt vv ty tm Hty1) (map snd ps))
+  (vv: val_vars pd vt)
+  (ty1: gen_type b)
+  (Hty1 : @gen_typed gamma b (gen_match tm ty ps) ty1)
+  (Hty2: @gen_typed gamma b 
+    match compile_bare_single b (rewriteT tm) ty
+      (map (fun x => (fst x, gen_rewrite (snd x))) ps)
+    with
+    | Some t2 => t2
+    | None => gen_match tm ty ps
+    end ty1)
+  (Hwf: gen_name_wf (gen_match tm ty ps)):
+  gen_rep gamma_valid pd pdf pf vt vv ty1
+    match
+    compile_bare_single b (rewriteT tm) ty
+      (map (fun x => (fst x, gen_rewrite (snd x))) ps)
+    with
+    | Some t2 => t2
+    | None => gen_match tm ty ps
+    end Hty2 = 
+  gen_rep gamma_valid pd pdf pf vt vv ty1 (gen_match tm ty ps) Hty1.
+Proof.
+  revert Hty2.
+  destruct (compile_bare_single b (rewriteT tm) ty
+    (map (fun x : pattern * gen_term b => (fst x, gen_rewrite (snd x))) ps)) as [t2|] eqn : Hcomp;
+  [|intros; apply gen_rep_irrel].
+  intros Hty2.
+  (*First set of typing results*)
+  assert (Hty1':=Hty1).
+  apply gen_match_typed_inv in Hty1'.
+  destruct Hty1' as [Hty1' [Hallps _]].
+  apply Forall_and_inv in Hallps.
+  destruct Hallps as [Hallpats Halltms].
+  erewrite gen_match_rep with (Hty1:=Hty1')(Hpats1:=Hallpats)(Hpats2:=Halltms); auto.
+  (*Why we needed wf*)
+  assert (Hdisj: disj (map fst (tm_fv (rewriteT tm)))
+  (map fst
+      (big_union vsymbol_eq_dec pat_fv
+        (map fst
+            (map (fun x => (fst x, gen_rewrite (snd x))) ps))))).
+  {
+    rewrite map_map. simpl.
+    (*Now use wf assumption*)
+    rewrite gen_name_wf_eq in Hwf.
+    rewrite gen_match_bnd, gen_match_fv in Hwf.
+    destruct Hwf as [_ Hwf].
+    eapply disj_sublist2.
+    { apply sublist_map. eapply rewriteT_fv; eauto. }
+    eapply disj_sublist_lr. apply Hwf.
+    - (*Prove fv sublist*)
+      simpl. 
+      intros x Hinx. rewrite in_map_union. auto.
+    - (*Prove bnd sublist*)
+      simpl. rewrite map_app, concat_map, map_map.
+      intros x. rewrite in_map_big_union with (eq_dec1:=string_dec).
+      rewrite in_app_iff, in_concat. simpl_set. intros [p [Hinp Hinx]].
+      right.
+      rewrite in_map_iff in Hinp. destruct Hinp as [pt [Hp Hinpt]].
+      subst p. eexists. split.
+      + rewrite in_map_iff. exists pt. split; [reflexivity| auto].
+      + rewrite map_app, in_app_iff; auto.
+  }
+  (*Typing results we need*)
+  assert (Htyr: term_has_type gamma (rewriteT tm) ty). {
+    apply rewriteT_typed; auto.
+  }
+  assert (Hpsr: Forall (fun p => pattern_has_type gamma (fst p) ty)
+    (map (fun x => (fst x, gen_rewrite (snd x))) ps)).
+  {
+    rewrite Forall_map. auto.
+  }
+  assert (Htsr: Forall (fun t => @gen_typed gamma b (snd t) ty1)
+  (map (fun x => (fst x, gen_rewrite (snd x))) ps)).
+  {
+    rewrite Forall_map; simpl. revert Halltms.
+    apply Forall_impl. intros a. apply gen_rewrite_typed; auto. 
+  }
+  apply wf_genmatch in Hwf. destruct Hwf as [Hwf1 Hwfall].
+  (*Use correctness of pat match compilation*)
+  eapply (compile_bare_single_spec2 gamma_valid pd pdf pf vt vv
+    b ty1) with (Hty:=Htyr) (Htyps1:=Hpsr) (Htyps2:=Htsr)
+    (Htym:=Hty2) in Hcomp; [|assumption].
+  simpl in Hcomp.
+  rewrite <- Hcomp; clear Hcomp.
+  (*Now prove [match_rep] equivalent by IHps*)
+  rewrite IHtm with (Hty1:=Hty1') by assumption.
+  rewrite Forall_map in IHps.
+  rewrite !match_rep_equiv. apply match_rep_ext.
+  + rewrite map_map. reflexivity.
+  + apply Forall2_flip, Forall2_map_iff.
+    revert IHps Hwfall. rewrite !Forall_forall; clear; intros Hall1 Hall2 x Hinx.
+    intros. apply Hall1; auto.
+Qed.
+
+(*Part 2 : Semantics*)
 Lemma rewrite_rep {gamma} (gamma_valid: valid_context gamma)
   (pd: pi_dom) (pdf: pi_dom_full gamma pd)
   (pf: pi_funpred gamma_valid pd pdf)
@@ -658,12 +1037,12 @@ Lemma rewrite_rep {gamma} (gamma_valid: valid_context gamma)
   t f:
   (forall (vv: val_vars pd vt) ty (Hty1: term_has_type gamma t ty)
     (Hty2: term_has_type gamma (rewriteT t) ty)
-    (Hwf: term_wf t),
+    (Hwf: term_name_wf t),
     term_rep gamma_valid pd pdf vt pf vv (rewriteT t) ty Hty2 =
     term_rep gamma_valid pd pdf vt pf vv t ty Hty1) /\
   (forall (vv: val_vars pd vt) (Hty1: formula_typed gamma f)
     (Hty2: formula_typed gamma (rewriteF f))
-    (Hwf: fmla_wf f),
+    (Hwf: fmla_name_wf f),
     formula_rep gamma_valid pd pdf vt pf vv (rewriteF f)  Hty2 =
     formula_rep gamma_valid pd pdf vt pf vv f Hty1).
 Proof.
@@ -680,88 +1059,142 @@ Proof.
     rewrite map_nth_inbound with (d2:=tm_d) by auto.
     intros Hty3 Hty4.
     rewrite Forall_nth in IH; apply IH; auto.
-    pose proof (wf_tfun Hwf) as IHwf.
-    rewrite Forall_nth in IHwf.
-    apply IHwf; auto.
+    apply (@wf_genfun true) in Hwf.
+    rewrite Forall_nth in Hwf.
+    apply Hwf; auto.
   - (*Tlet*)
     intros tm1 ty tm2 IH1 IH2 vv ty1 Hty1 Hty2 Hwf.
     simpl_rep_full.
-    pose proof (wf_tlet Hwf) as [Hwf1 Hwf2].
+    pose proof (wf_genlet true Hwf) as [Hwf1 Hwf2].
     rewrite IH1 with (Hty1:=(proj1' (ty_let_inv Hty1))) by auto.
     apply IH2; auto.
   - (*Tif*)
     intros f t1 t2 IH1 IH2 IH3 vv ty Hty1 Hty2 Hwf.
-    apply wf_tif in Hwf.
+    apply (wf_genif true) in Hwf.
     destruct Hwf as [Hwf1 [Hwf2 Hwf3]].
     simpl_rep_full.
     erewrite IH1, IH2, IH3 by auto. reflexivity.
   - (*Tmatch - the interesting case*)
     intros tm ty ps IHtm IHps vv ty1 Hty1 Hty2 Hwf.
-    revert Hty2.
-    destruct (compile_bare_single true (rewriteT tm) ty
-      (map (fun x : pattern * term => (fst x, rewriteT (snd x))) ps)) as [t2|] eqn : Hcomp;
-    [|intros; apply term_rep_irrel].
-    intros Hty2.
+    apply (rewrite_rep_match_case true); auto.
+  - (*Teps*)
+    intros f v IH vv t Hty1 Hty2 Hwf. 
     simpl_rep_full.
-    (*Why we needed wf*)
-    assert (Hdisj: disj (map fst (tm_fv (rewriteT tm)))
-    (map fst
-        (big_union vsymbol_eq_dec pat_fv
-          (map fst
-              (map (fun x : pattern * term => (fst x, rewriteT (snd x))) ps))))).
-    {
+    apply wf_teps in Hwf.
+    f_equal. repeat (apply functional_extensionality_dep; intros).
+    rewrite IH with (Hty1:=(proj1' (ty_eps_inv Hty1))); auto.
+    do 4 f_equal. apply UIP_dec, sort_eq_dec.
+  - (*Fpred*)
+    intros f1 tys tms IH vv Hty1 Hty2 Hwf.
+    simpl_rep_full.
+    f_equal.
+    apply get_arg_list_ext; [rewrite map_length; auto|].
+    intros i. rewrite map_length. intros Hi ty1.
+    rewrite map_nth_inbound with (d2:=tm_d) by auto.
+    intros Hty3 Hty4.
+    rewrite Forall_nth in IH; apply IH; auto.
+    apply (@wf_genfun false) in Hwf.
+    rewrite Forall_nth in Hwf.
+    apply Hwf; auto.
+  - (*Fquant*)
+    intros q v f IH vv Hty1 Hty2 Hwf.
+    simpl. apply wf_fquant in Hwf.
+    destruct q; simpl_rep_full;
+    apply all_dec_eq;
+    setoid_rewrite IH; try reflexivity; auto.
+  - (*Feq*)
+    intros ty t1 t2 IH1 IH2 vv Hty1 Hty2 Hwf.
+    simpl_rep_full. apply all_dec_eq.
+    apply wf_feq in Hwf. destruct Hwf.
+    erewrite IH1, IH2; [reflexivity| |]; auto.
+  - (*Fbinop*)
+    intros b f1 f2 IH1 IH2 vv Hty1 Hty2 Hwf.
+    apply wf_fbinop in Hwf; destruct Hwf.
+    simpl_rep_full. erewrite IH1, IH2; [reflexivity| |]; auto.
+  - (*Fnot*)
+    intros f IH vv Hty1 Hty2 Hwf.
+    simpl_rep_full. apply wf_fnot in Hwf. f_equal; apply IH; auto.
+  - (*Flet*)
+    intros tm1 ty tm2 IH1 IH2 vv Hty1 Hty2 Hwf.
+    simpl_rep_full.
+    pose proof (wf_genlet false Hwf) as [Hwf1 Hwf2].
+    rewrite IH1 with (Hty1:=(proj1' (typed_let_inv Hty1))) by auto.
+    apply IH2; auto.
+  - (*Fif*)
+    intros f t1 t2 IH1 IH2 IH3 vv Hty1 Hty2 Hwf.
+    apply (wf_genif false) in Hwf.
+    destruct Hwf as [Hwf1 [Hwf2 Hwf3]].
+    simpl_rep_full.
+    erewrite IH1, IH2, IH3 by auto. reflexivity.
+  - (*Fmatch*)
+    intros tm ty ps IHtm IHps vv Hty1 Hty2 Hwf.
+    apply (rewrite_rep_match_case false) with (ty1:=tt); auto.
+    revert IHps. apply Forall_impl.
+    simpl. intros. auto.
+Qed.
 
-    }
-    
-    pose proof (compile_bare_single_spec2 gamma_valid pd pdf pf vt vv true
-      ty1 _ _ _ _ _ _ _ _ Hty2 Hcomp).
-    Search compile_bare_single.
-    2: {
+Definition rewriteT_rep {gamma} (gamma_valid: valid_context gamma)
+  (pd: pi_dom) (pdf: pi_dom_full gamma pd)
+  (pf: pi_funpred gamma_valid pd pdf)
+  (vt: val_typevar) (vv: val_vars pd vt)
+  t ty (Hty1: term_has_type gamma t ty)
+  (Hty2: term_has_type gamma (rewriteT t) ty)
+  (Hwf: term_name_wf t):=
+  proj_tm (rewrite_rep gamma_valid pd pdf pf vt) t vv ty Hty1 Hty2 Hwf.
 
-    }
+Definition rewriteF_rep {gamma} (gamma_valid: valid_context gamma)
+  (pd: pi_dom) (pdf: pi_dom_full gamma pd)
+  (pf: pi_funpred gamma_valid pd pdf)
+  (vt: val_typevar) (vv: val_vars pd vt)
+  f (Hty1: formula_typed gamma f)
+  (Hty2: formula_typed gamma (rewriteF f))
+  (Hwf: fmla_name_wf f):=
+  proj_fmla (rewrite_rep gamma_valid pd pdf pf vt) f vv Hty1 Hty2 Hwf.
 
-    erewrite IH2 by auto.
-    
-    
+(*And combine with alpha to remove the wf*)
 
-    (*1*)
-
-
-    Search term_wf.
-    
-     intros Hi ty1 Hty3 Hty4.
-    revert Hty3.
-    rewrite map_nth_inbound with (d2:=tm_d).
-    Search fun_arg_list.
-    apply fun_arg_list_ext.
-    Search get_arg_list.
-    Print term_wf.
-  
-  
-  
-   intros; apply term_rep_irrel.
-
-
-Lemma rewrite_typed {gamma} (gamma_valid: valid_context gamma) t f:
-  (forall ty (Hty: term_has_type gamma t ty),
-    term_has_type gamma (rewriteT t) ty) /\
-  (forall (Hty: formula_typed gamma f),
-    formula_typed gamma (rewriteF f)).
-
-
-(*3: Simple patterns*)
-
-
-    
-     t ty:
-  term_has_type gamma t ty ->
-  term_has_type gamma (rewriteT t) ty.
+Corollary rewriteT_rep' {gamma} (gamma_valid: valid_context gamma)
+  (pd: pi_dom) (pdf: pi_dom_full gamma pd)
+  (pf: pi_funpred gamma_valid pd pdf)
+  (vt: val_typevar) (vv: val_vars pd vt)
+  t ty (Hty1: term_has_type gamma t ty)
+  (Hty2: term_has_type gamma (rewriteT' t) ty):
+  term_rep gamma_valid pd pdf vt pf vv (rewriteT' t) ty Hty2 =
+  term_rep gamma_valid pd pdf vt pf vv t ty Hty1.
 Proof.
-  unfold rewriteT.
+  unfold rewriteT'.
+  erewrite rewriteT_rep by apply a_convert_all_t_name_wf.
+  rewrite <- a_convert_all_t_rep. reflexivity.
+Qed.
 
-Lemma compile_match_sound: sound_trans compile_match.
+Corollary rewriteF_rep' {gamma} (gamma_valid: valid_context gamma)
+  (pd: pi_dom) (pdf: pi_dom_full gamma pd)
+  (pf: pi_funpred gamma_valid pd pdf)
+  (vt: val_typevar) (vv: val_vars pd vt)
+  f (Hty1: formula_typed gamma f)
+  (Hty2: formula_typed gamma (rewriteF' f)):
+  formula_rep gamma_valid pd pdf vt pf vv (rewriteF' f) Hty2 =
+  formula_rep gamma_valid pd pdf vt pf vv f Hty1.
+Proof.
+  unfold rewriteF'.
+  erewrite rewriteF_rep by apply a_convert_all_f_name_wf.
+  rewrite <- a_convert_all_f_rep. reflexivity.
+Qed.
+
+(*And therefore, the transformation is sound*)
+Theorem compile_match_valid: sound_trans compile_match.
 Proof.
   unfold compile_match.
-  apply trans_map_sound. *)
+  apply trans_map_sound.
+  - intros gamma t ty gamma_valid Hty.
+    apply rewriteT_typed; auto.
+    apply a_convert_all_t_ty; auto.
+  - intros gamma f gamma_valid Hty.
+    apply rewriteF_typed; auto.
+    apply a_convert_all_f_typed; auto.
+  - intros; symmetry; apply rewriteT_rep'.
+  - intros; symmetry; apply rewriteF_rep'.
+Qed.
 
+(*Part 3: Simple patterns*)
 
